Test/civl/lock-introduced.bpl
@@ -92,7 +92,7 @@ procedure {:yields} {:layer 1} {:refines "AtomicLowerLeave"} LowerLeave()
   yield;
 }
 
-procedure {:layer 1} {:inline 1} SetLock(v: X)
+procedure {:intro} {:layer 1} SetLock(v: X)
 modifies lock;
 { lock := v; }
 
