Test/civl/par-intro-bug.bpl
@@ -3,15 +3,14 @@
 
 var {:layer 0} x : int;
 
-procedure {:layer 0} set_x(v: int)
-ensures {:layer 0} x == v;	 
+procedure {:intro} {:layer 0} set_x(v: int)
 modifies x;
 {
   x := v;
-}	
+}
 
 procedure {:yields} {:layer 0} yield_set_x(v: int)
-ensures {:layer 0} x == v;	
+ensures {:layer 0} x == v;
 {
   yield;
 	call set_x(v);
@@ -21,4 +20,4 @@ procedure {:yields} {:layer 0} main()
 {
   par yield_set_x(4) | yield_set_x(3);
 	assert {:layer 0} false;
-}	
+}
