Test/civl/ticket.bpl
@@ -141,12 +141,12 @@ procedure {:right} {:layer 2} AtomicGetTicketAbstract ({:linear "tid"} tid: X) r
 modifies T;
 { assume !T[m]; T[m] := true; }
 
-procedure {:yields} {:layer 1} {:refines "AtomicGetTicketAbstract"} GetTicketAbstract ({:linear "tid"} tid: X) returns (blah: int)
+procedure {:yields} {:layer 1} {:refines "AtomicGetTicketAbstract"} GetTicketAbstract ({:linear "tid"} tid: X) returns (m: int)
 requires {:layer 1} Inv1(T, t);
 ensures  {:layer 1} Inv1(T, t);
 {
   par Yield1();
-  call blah := GetTicket(tid);
+  call m := GetTicket(tid);
   par Yield1();
 }
 
